Rustan's lemmas to fix ARN timeouts

src/KMS/KMSUtils.dfy
@@ -11,9 +11,7 @@ module {:extern "KMSUtils"} KMSUtils {
 
   const MAX_GRANT_TOKENS := 10
 
-  //FIXME: Ideally, we would use this restrictive subtype definition. Right now though, it results in verification timeouts.
-  //type CustomerMasterKey = s: string | ValidFormatCMK(s) witness "alias/ExampleAlias"
-  type CustomerMasterKey = string
+  type CustomerMasterKey = s: string | ValidFormatCMK(s) witness CreateValidFormatCMKAlias("ExampleAlias")
 
   predicate method ValidFormatCMK(cmk: string) {
     ValidFormatCMKKeyARN(cmk) || ValidFormatCMKAlias(cmk) || ValidFormatCMKAliasARN(cmk)
@@ -34,6 +32,84 @@ module {:extern "KMSUtils"} KMSUtils {
     0 < |cmk| <= 2048 && |components| == 6 && components[0] == "arn" && components[2] == "kms" && Split(components[5], '/')[0] == "alias"
   }
 
+  function method CreateValidFormatCMKAlias(y: string): (s: string)
+    requires |"alias/"| + |y| <= 2048 && '/' !in y
+    ensures s == "alias/" + y && ValidFormatCMKAlias(s)
+  {
+    var s := "alias/" + y;
+    ghost var delim := '/';
+    calc {
+      Split(s, delim);
+    ==  { AboutSplit0(s, delim, "alias"); }
+      ["alias"] + Split(s[6..], delim);
+    ==  { assert s[6..] == y; }
+      ["alias"] + Split(y, delim);
+    ==  { AboutSplit1(y, delim); }
+      ["alias"] + [y];
+    ==  // concatenation of singleton sequences
+      ["alias", y];
+    }
+    s
+  }
+
+  //TODO: CreateValidFormatCMKAliasARN
+
+  function method CreateValidFormatCMKKeyARN(aws: string, region: string, account_id: string, y: string): (s: CustomerMasterKey)
+    requires ':' !in aws && ':' !in region && ':' !in account_id && ':' !in y
+    requires |aws| <= 10 && |region| <= 1000 && |account_id| == 12 && |y| == 36
+    ensures s == "arn:" + aws + ":kms:" + region + ":" + account_id + ":key/" + y
+    ensures ValidFormatCMKKeyARN(s)
+  {
+    var arn, kms, key := "arn", "kms", "key";
+    var keyY := key + "/" + y;
+    var s := arn + ":" + aws + ":" + kms + ":" + region + ":" + account_id + ":" + keyY;
+    // To prove ValidFormatCMKKeyARN, we need to prove three things. The first is easy:
+    assert 0 < |s| <= 2048;
+    // The second is the most complicated, because we need to reason about what
+    // Split(s, ':') returns. If you're reading this line by line, you may want to
+    // look at the third part next, because its ingredients are the same as in the second
+    // part, but simpler.
+    ghost var components := Split(s, ':');
+    assert components == [arn, aws, kms, region, account_id, keyY] by {
+      var delim := ':';
+      calc {
+        Split(s, delim);
+      ==  { AboutSplit0(s, delim, arn); }
+        [arn] + Split(s[|arn|+1..], delim);
+      ==  { AboutSplit0(s[|arn|+1..], delim, aws); }
+        [arn] + ([aws] + Split(s[|arn|+1..][|aws|+1..], delim));
+      ==  { assert s[|arn|+1..][|aws|+1..] == s[|arn|+|aws|+2..]; }
+        [arn, aws] + Split(s[|arn|+|aws|+2..], delim);
+      ==  { AboutSplit0(s[|arn|+|aws|+2..], delim, kms); }
+        [arn, aws] + ([kms] + Split(s[|arn|+|aws|+2..][|kms|+1..], delim));
+      ==  { assert s[|arn|+|aws|+2..][|kms|+1..] == s[|arn|+|aws|+|kms|+3..]; }
+        [arn, aws, kms] + Split(s[|arn|+|aws|+|kms|+3..], delim);
+      ==  { AboutSplit0(s[|arn|+|aws|+|kms|+3..], delim, region); }
+        [arn, aws, kms] + ([region] + Split(s[|arn|+|aws|+|kms|+3..][|region|+1..], delim));
+      ==  { assert s[|arn|+|aws|+|kms|+3..][|region|+1..] == s[|arn|+|aws|+|kms|+|region|+4..]; }
+        [arn, aws, kms, region] + Split(s[|arn|+|aws|+|kms|+|region|+4..], delim);
+      ==  { AboutSplit0(s[|arn|+|aws|+|kms|+|region|+4..], delim, account_id); }
+        [arn, aws, kms, region] + ([account_id] + Split(s[|arn|+|aws|+|kms|+|region|+4..][|account_id|+1..], delim));
+      ==  { assert s[|arn|+|aws|+|kms|+|region|+4..][|account_id|+1..] == s[|arn|+|aws|+|kms|+|region|+|account_id|+5..]; }
+        [arn, aws, kms, region, account_id] + Split(s[|arn|+|aws|+|kms|+|region|+|account_id|+5..], delim);
+      ==  { assert s[|arn|+|aws|+|kms|+|region|+|account_id|+5..] == keyY; }
+        [arn, aws, kms, region, account_id] + Split(keyY, delim);
+      ==  { AboutSplit1(keyY, delim); }
+        [arn, aws, kms, region, account_id] + [keyY];
+      ==
+        [arn, aws, kms, region, account_id, keyY];
+      }
+    }
+    // The third is like a shorter version of the second part.
+    ghost var kcomponents := Split(keyY, '/');
+    assert kcomponents[0] == key by {
+      AboutSplit0(keyY, '/', key);
+    }
+    // And after proving those three things, we have proved that s satisfies ValidFormatCMKKeyARN,
+    // so we are ready to return it:
+    s
+  }
+  
   type GrantToken = s: string | 0 < |s| <= 8192 witness "witness"
 
   trait ClientSupplier {
