src/Main.dfy
@@ -66,6 +66,7 @@ module Main {
     }
 
     var generatorStr := "arn:aws:kms:us-west-2:658956600833:key/b3537ef1-d8dc-4780-9f5a-55776cbb2f7f";
+    assert generatorStr == KMSUtils.CreateValidFormatCMKKeyARN("aws", "us-west-2", "658956600833", "b3537ef1-d8dc-4780-9f5a-55776cbb2f7f");
     var generator: KMSUtils.CustomerMasterKey := generatorStr;
     var clientSupplier := new KMSUtils.DefaultClientSupplier();
     var keyring := new KMSKeyring.KMSKeyring(clientSupplier, [], Some(generator), []);
